rearrange MarshallingModel so that stuff is in Marshalling file instead

Impl/Marshalling.i.dfy
@@ -1,4 +1,11 @@
-include "MarshallingModel.i.dfy"
+include "../lib/Marshalling/GenericMarshalling.i.dfy"
+include "../PivotBetree/PivotBetreeSpec.i.dfy"
+include "../lib/Base/Message.i.dfy"
+include "../lib/Base/Crypto.s.dfy"
+include "../lib/Base/Option.s.dfy"
+include "../BlockCacheSystem/BlockCache.i.dfy"
+include "KVList.i.dfy"
+
 //
 // Raises ImpLMarshallingModel by converting indirection table sectors
 // up from IndirectionTableModel.IndirectionTable to
@@ -13,19 +20,23 @@ include "MarshallingModel.i.dfy"
 //
 
 module Marshalling {
-  import IMM = ImplMarshallingModel
-  import IM = StateModel
   import opened GenericMarshalling
   import opened Options
   import opened NativeTypes
   import opened Sequences
   import opened BucketsLib
+  import opened BucketWeights
   import BC = BetreeGraphBlockCache
   import BT = PivotBetreeSpec`Internal
   import M = ValueMessage`Internal
   import Pivots = PivotsLib
   import KVList
-  import IndirectionTableModel
+  import Keyspace = Lexicographic_Byte_Order
+  import SeqComparison
+  import opened Bounds
+  import LBAType
+  import ReferenceType`Internal
+  import Crypto
 
   type Reference = BC.Reference
   type LBA = BC.LBA
@@ -33,63 +44,305 @@ module Marshalling {
   type Sector = BC.Sector
   type Node = BT.G.Node
 
+  /////// Grammar
+
+  function method BucketGrammar() : G
+  ensures ValidGrammar(BucketGrammar())
+  {
+    GTuple([
+      GKeyArray,
+      GMessageArray
+    ])
+  }
+
+  function method PivotNodeGrammar() : G
+  ensures ValidGrammar(PivotNodeGrammar())
+  {
+    GTuple([
+        GKeyArray, // pivots
+        GUint64Array, // children
+        GArray(BucketGrammar()) 
+    ])
+  }
+
+  function method IndirectionTableGrammar() : G
+  ensures ValidGrammar(IndirectionTableGrammar())
+  {
+    // (Reference, address, len, successor-list) triples
+    GArray(GTuple([GUint64, GUint64, GUint64, GUint64Array]))
+  }
+
+  function method SectorGrammar() : G
+  ensures ValidGrammar(SectorGrammar())
+  {
+    GTaggedUnion([IndirectionTableGrammar(), PivotNodeGrammar()])    
+  }
+
   /////// Conversion to PivotNode
 
-  /*function valToIndirectionTable(v: V) : (s : Option<BC.IndirectionTable>)
-  requires ValidVal(v)
-  requires ValInGrammar(v, IndirectionTableModel.IndirectionTableGrammar())
-  ensures s.Some? ==> BC.WFCompleteIndirectionTable(s.value)
+  predicate isStrictlySortedKeySeqIterate(a: seq<Key>, i: int)
+  requires 1 <= i <= |a|
+  decreases |a| - i
+  ensures isStrictlySortedKeySeqIterate(a, i) <==> Keyspace.IsStrictlySorted(a[i-1..])
   {
-    MapOption(IndirectionTableModel.valToIndirectionTable(v), IM.IIndirectionTable)
-  }*/
+    Keyspace.reveal_IsStrictlySorted();
 
-  function {:fuel ValInGrammar,2} valToBucket(v: V, pivotTable: seq<Key>, i: int) : (s : Option<map<Key, Message>>)
+    if i == |a| then (
+      true
+    ) else (
+      if (Keyspace.lt(a[i-1], a[i])) then (
+        isStrictlySortedKeySeqIterate(a, i+1)
+      ) else (
+        false
+      )
+    )
+  }
+
+
+  predicate {:opaque} isStrictlySortedKeySeq(a: seq<Key>)
+  ensures isStrictlySortedKeySeq(a) <==> Keyspace.IsStrictlySorted(a)
+  {
+    Keyspace.reveal_IsStrictlySorted();
+
+    if |a| >= 2 then (
+      isStrictlySortedKeySeqIterate(a, 1)
+    ) else (
+      true
+    )
+  }
+
+  function valToStrictlySortedKeySeq(v: V) : (s : Option<seq<Key>>)
   requires ValidVal(v)
-  requires ValInGrammar(v, IMM.BucketGrammar())
+  requires ValInGrammar(v, GKeyArray)
+  ensures s.Some? ==> Keyspace.IsStrictlySorted(s.value)
+  ensures s.Some? ==> |s.value| == |v.baa|
+  decreases |v.baa|
+  {
+    if isStrictlySortedKeySeq(v.baa) then
+      var blah : seq<Key> := v.baa;
+      Some(v.baa)
+    else
+      None
+  }
+
+  function valToPivots(v: V) : (s : Option<seq<Key>>)
+  requires ValidVal(v)
+  requires ValInGrammar(v, GKeyArray)
+  ensures s.Some? ==> Pivots.WFPivots(s.value)
+  ensures s.Some? ==> |s.value| == |v.baa|
+  {
+    var s := valToStrictlySortedKeySeq(v);
+    if s.Some? && (|s.value| > 0 ==> |s.value[0]| != 0) then (
+      if |s.value| > 0 then (
+        SeqComparison.reveal_lte();
+        Keyspace.IsNotMinimum([], s.value[0]);
+        s
+      ) else (
+        s
+      )
+    ) else (
+      None
+    )
+  }
+
+  function {:fuel ValInGrammar,2} valToMessageSeq(v: V) : (s : Option<seq<Message>>)
+  requires ValidVal(v)
+  requires ValInGrammar(v, GMessageArray)
+  ensures s.Some? ==> forall i | 0 <= i < |s.value| :: s.value[i] != M.IdentityMessage()
+  ensures s.Some? ==> |s.value| == |v.ma|
+  decreases |v.ma|
+  {
+    assert forall i | 0 <= i < |v.ma| :: ValidMessage(v.ma[i]);
+    Some(v.ma)
+  }
+
+  function {:fuel ValInGrammar,2} valToBucket(v: V, pivotTable: seq<Key>, i: int) : (s : Option<KVList.Kvl>)
+  requires ValidVal(v)
+  requires ValInGrammar(v, BucketGrammar())
   requires Pivots.WFPivots(pivotTable)
   requires 0 <= i <= |pivotTable|
   {
-    MapOption(IMM.valToBucket(v, pivotTable, i), KVList.I)
+    var keys := valToStrictlySortedKeySeq(v.t[0]);
+    var values := valToMessageSeq(v.t[1]);
+
+    if keys.Some? && values.Some? then (
+      var kvl := KVList.Kvl(keys.value, values.value);
+
+      if KVList.WF(kvl) && WFBucketAt(KVList.I(kvl), pivotTable, i) then
+        Some(kvl)
+      else
+        None
+    ) else (
+      None
+    )
   }
 
-  function valToBuckets(a: seq<V>, pivotTable: seq<Key>) : (s : Option<seq<map<Key, Message>>>)
+  function valToBuckets(a: seq<V>, pivotTable: seq<Key>) : (s : Option<seq<Bucket>>)
   requires Pivots.WFPivots(pivotTable)
   requires forall i | 0 <= i < |a| :: ValidVal(a[i])
-  requires forall i | 0 <= i < |a| :: ValInGrammar(a[i], IMM.BucketGrammar())
+  requires forall i | 0 <= i < |a| :: ValInGrammar(a[i], BucketGrammar())
   requires |a| <= |pivotTable| + 1
   ensures s.Some? ==> |s.value| == |a|
   ensures s.Some? ==> forall i | 0 <= i < |s.value| :: WFBucketAt(s.value[i], pivotTable, i)
   {
-    IMM.valToBuckets(a, pivotTable)
+    if |a| == 0 then
+      Some([])
+    else (
+      match valToBuckets(DropLast(a), pivotTable) {
+        case None => None
+        case Some(pref) => (
+          match valToBucket(Last(a), pivotTable, |pref|) {
+            case Some(bucket) => Some(pref + [KVList.I(bucket)])
+            case None => None
+          }
+        )
+      }
+    )
+  }
+
+  function method valToChildren(v: V) : Option<seq<Reference>>
+  requires ValInGrammar(v, GUint64Array)
+  {
+    Some(v.ua)
   }
 
   function {:fuel ValInGrammar,2} valToNode(v: V) : (s : Option<Node>)
   requires ValidVal(v)
-  requires ValInGrammar(v, IMM.PivotNodeGrammar())
+  requires ValInGrammar(v, PivotNodeGrammar())
+  // Pivots.NumBuckets(node.pivotTable) == |node.buckets|
   ensures s.Some? ==> BT.WFNode(s.value)
   {
-    MapOption(IMM.valToNode(v), IM.INode)
+    assert ValidVal(v.t[0]);
+    assert ValidVal(v.t[1]);
+    assert ValidVal(v.t[2]);
+    var pivots_len := |v.t[0].baa| as uint64;
+    var children_len := |v.t[1].ua| as uint64;
+    var buckets_len := |v.t[2].a| as uint64;
+
+    if (
+       && pivots_len <= MaxNumChildrenUint64() - 1
+       && (children_len == 0 || children_len == pivots_len + 1)
+       && buckets_len == pivots_len + 1
+    ) then (
+      assert ValidVal(v.t[0]);
+      match valToPivots(v.t[0]) {
+        case None => None
+        case Some(pivots) => (
+          match valToChildren(v.t[1]) {
+            case None => None
+            case Some(children) => (
+              assert ValidVal(v.t[2]);
+              match valToBuckets(v.t[2].a, pivots) {
+                case None => None
+                case Some(buckets) => (
+                  if WeightBucketList(buckets) <= MaxTotalBucketWeight() then (
+                    var node := BT.G.Node(
+                      pivots,
+                      if |children| == 0 then None else Some(children),
+                      buckets);
+                    Some(node)
+                  ) else (
+                    None
+                  )
+                )
+              }
+            )
+          }
+        )
+      }
+    ) else (
+      None
+    )
   }
 
-  function valToSector(v: V) : (s : Option<BC.Sector>)
-  requires ValidVal(v)
-  requires ValInGrammar(v, IMM.SectorGrammar())
+  function {:fuel ValInGrammar,3} valToIndirectionTableMaps(a: seq<V>) : (s : Option<BC.IndirectionTable>)
+  requires |a| <= IndirectionTableMaxSize()
+  requires forall i | 0 <= i < |a| :: ValidVal(a[i])
+  requires forall i | 0 <= i < |a| :: ValInGrammar(a[i], GTuple([GUint64, GUint64, GUint64, GUint64Array]))
+  ensures s.Some? ==> |s.value.graph| as int == |a|
+  ensures s.Some? ==> s.value.graph.Keys == s.value.locs.Keys
+  ensures s.Some? ==> forall v | v in s.value.locs.Values :: BC.ValidLocationForNode(v)
+  ensures s.Some? ==> forall ref | ref in s.value.graph :: |s.value.graph[ref]| <= MaxNumChildren()
   {
-    MapOption(IMM.valToSector(v), IM.ISector)
+    if |a| == 0 then
+      Some(BC.IndirectionTable(map[], map[]))
+    else (
+      var res := valToIndirectionTableMaps(DropLast(a));
+      match res {
+        case Some(table) => (
+          var tuple := Last(a);
+          var ref := tuple.t[0].u;
+          var lba := tuple.t[1].u;
+          var len := tuple.t[2].u;
+          var succs := Some(tuple.t[3].ua);
+          match succs {
+            case None => None
+            case Some(succs) => (
+              var loc := LBAType.Location(lba, len);
+              if ref in table.graph || lba == 0 || !LBAType.ValidLocation(loc) || |succs| as int > MaxNumChildren() then (
+                None
+              ) else (
+                Some(BC.IndirectionTable(table.locs[ref := loc], table.graph[ref := succs]))
+              )
+            )
+          }
+        )
+        case None => None
+      }
+    )
   }
 
+  function valToIndirectionTable(v: V) : (s : Option<BC.IndirectionTable>)
+  requires ValidVal(v)
+  requires ValInGrammar(v, IndirectionTableGrammar())
+  ensures s.Some? ==> BC.WFCompleteIndirectionTable(s.value)
+  {
+    if |v.a| <= IndirectionTableMaxSize() then (
+      var t := valToIndirectionTableMaps(v.a);
+      match t {
+        case Some(res) => (
+          if BT.G.Root() in res.graph && BC.GraphClosed(res.graph) then (
+            Some(res)
+          ) else (
+            None
+          )
+        )
+        case None => None
+      }
+    ) else (
+      None
+    )
+  }
+
+  function valToSector(v: V) : (s : Option<Sector>)
+  requires ValidVal(v)
+  requires ValInGrammar(v, SectorGrammar())
+  {
+    if v.c == 0 then (
+      match valToIndirectionTable(v.val) {
+        case Some(s) => Some(BC.SectorIndirectionTable(s))
+        case None => None
+      }
+    ) else (
+      match valToNode(v.val) {
+        case Some(s) => Some(BC.SectorBlock(s))
+        case None => None
+      }
+    )
+  }
 
   /////// Marshalling and de-marshalling
 
-  function {:opaque} parseSector(data: seq<byte>) : (s : Option<BC.Sector>)
+  function {:opaque} parseSector(data: seq<byte>) : (s : Option<Sector>)
+  //ensures s.Some? ==> SM.WFSector(s.value)
   {
-    MapOption(IMM.parseSector(data), IM.ISector)
-  }
-
-  /////// Marshalling and de-marshalling with checksums
-
-  function {:opaque} parseCheckedSector(data: seq<byte>) : (s : Option<BC.Sector>)
-  {
-    MapOption(IMM.parseCheckedSector(data), IM.ISector)
+    if |data| < 0x1_0000_0000_0000_0000 then (
+      match parse_Val(data, SectorGrammar()).0 {
+        case Some(v) => valToSector(v)
+        case None => None
+      }
+    ) else (
+      None
+    )
   }
 }
