Impl/MarshallingModel.i.dfy
@@ -1,12 +1,7 @@
-include "../lib/Marshalling/GenericMarshalling.i.dfy"
-include "../PivotBetree/PivotBetreeSpec.i.dfy"
-include "../lib/Base/Message.i.dfy"
+include "Marshalling.i.dfy"
 include "StateModel.i.dfy"
-include "../lib/Base/Crypto.s.dfy"
-include "../lib/Base/Option.s.dfy"
-include "../lib/Base/NativeArrays.s.dfy"
-include "../lib/DataStructures/MutableMapImpl.i.dfy"
-include "KVList.i.dfy"
+include "IndirectionTableModel.i.dfy"
+
 //
 // Parses bytes and returns the data structure (a Pivot-Node Sector) used by
 // the Model.
@@ -34,6 +29,7 @@ module ImplMarshallingModel {
   import NativeArrays
   import IndirectionTableModel
   import SeqComparison
+  import Marshalling
 
   import BT = PivotBetreeSpec`Internal
 
@@ -59,260 +55,11 @@ module ImplMarshallingModel {
   type Sector = SM.Sector
   type Node = SM.Node
 
-  /////// Grammar
-
-  function method BucketGrammar() : G
-  ensures ValidGrammar(BucketGrammar())
-  {
-    GTuple([
-      GKeyArray,
-      GMessageArray
-    ])
-  }
-
-  function method PivotNodeGrammar() : G
-  ensures ValidGrammar(PivotNodeGrammar())
-  {
-    GTuple([
-        GKeyArray, // pivots
-        GUint64Array, // children
-        GArray(BucketGrammar()) 
-    ])
-  }
-
-  function method SectorGrammar() : G
-  ensures ValidGrammar(SectorGrammar())
-  {
-    GTaggedUnion([IndirectionTableModel.IndirectionTableGrammar(), PivotNodeGrammar()])    
-  }
-
-  /////// Conversion to PivotNode
-
-  function method valToReference(v: V) : Reference
-  requires ValInGrammar(v, GUint64)
-  {
-    v.u
-  }
-
-  function method valToLBA(v: V) : LBA
-  requires ValInGrammar(v, GUint64)
-  {
-    v.u
-  }
-
-  function method valToChildren(v: V) : Option<seq<Reference>>
-  requires ValInGrammar(v, GUint64Array)
-  {
-    Some(v.ua)
-  }
-
-
-  function valToUint64Seq(v: V) : (s : seq<uint64>)
-  requires ValInGrammar(v, GUint64Array)
-  {
-    v.ua
-  }
-
-  predicate isStrictlySortedKeySeqIterate(a: seq<Key>, i: int)
-  requires 1 <= i <= |a|
-  decreases |a| - i
-  ensures isStrictlySortedKeySeqIterate(a, i) <==> Keyspace.IsStrictlySorted(a[i-1..])
-  {
-    Keyspace.reveal_IsStrictlySorted();
-
-    if i == |a| then (
-      true
-    ) else (
-      if (Keyspace.lt(a[i-1], a[i])) then (
-        isStrictlySortedKeySeqIterate(a, i+1)
-      ) else (
-        false
-      )
-    )
-  }
-
-  predicate {:opaque} isStrictlySortedKeySeq(a: seq<Key>)
-  ensures isStrictlySortedKeySeq(a) <==> Keyspace.IsStrictlySorted(a)
-  {
-    Keyspace.reveal_IsStrictlySorted();
-
-    if |a| >= 2 then (
-      isStrictlySortedKeySeqIterate(a, 1)
-    ) else (
-      true
-    )
-  }
-
-  function valToStrictlySortedKeySeq(v: V) : (s : Option<seq<Key>>)
-  requires ValidVal(v)
-  requires ValInGrammar(v, GKeyArray)
-  ensures s.Some? ==> Keyspace.IsStrictlySorted(s.value)
-  ensures s.Some? ==> |s.value| == |v.baa|
-  decreases |v.baa|
-  {
-    if isStrictlySortedKeySeq(v.baa) then
-      var blah : seq<Key> := v.baa;
-      Some(v.baa)
-    else
-      None
-  }
-
-  function valToPivots(v: V) : (s : Option<seq<Key>>)
-  requires ValidVal(v)
-  requires ValInGrammar(v, GKeyArray)
-  ensures s.Some? ==> Pivots.WFPivots(s.value)
-  ensures s.Some? ==> |s.value| == |v.baa|
-  {
-    var s := valToStrictlySortedKeySeq(v);
-    if s.Some? && (|s.value| > 0 ==> |s.value[0]| != 0) then (
-      if |s.value| > 0 then (
-        SeqComparison.reveal_lte();
-        Keyspace.IsNotMinimum([], s.value[0]);
-        s
-      ) else (
-        s
-      )
-    ) else (
-      None
-    )
-  }
-
-  function {:fuel ValInGrammar,2} valToMessageSeq(v: V) : (s : Option<seq<Message>>)
-  requires ValidVal(v)
-  requires ValInGrammar(v, GMessageArray)
-  ensures s.Some? ==> forall i | 0 <= i < |s.value| :: s.value[i] != M.IdentityMessage()
-  ensures s.Some? ==> |s.value| == |v.ma|
-  decreases |v.ma|
-  {
-    assert forall i | 0 <= i < |v.ma| :: ValidMessage(v.ma[i]);
-    Some(v.ma)
-  }
-
-  function {:fuel ValInGrammar,2} valToBucket(v: V, pivotTable: seq<Key>, i: int) : (s : Option<KVList.Kvl>)
-  requires ValidVal(v)
-  requires ValInGrammar(v, BucketGrammar())
-  requires Pivots.WFPivots(pivotTable)
-  requires 0 <= i <= |pivotTable|
-  {
-    var keys := valToStrictlySortedKeySeq(v.t[0]);
-    var values := valToMessageSeq(v.t[1]);
-
-    if keys.Some? && values.Some? then (
-      var kvl := KVList.Kvl(keys.value, values.value);
-
-      if KVList.WF(kvl) && WFBucketAt(KVList.I(kvl), pivotTable, i) then
-        Some(kvl)
-      else
-        None
-    ) else (
-      None
-    )
-  }
-
-  function IKVListOpt(table : Option<KVList.Kvl>): Option<map<Key, Message>>
-  requires table.Some? ==> KVList.WF(table.value)
-  {
-    if table.Some? then
-      Some(KVList.I(table.value))
-    else
-      None
-  }
-
-  function valToBuckets(a: seq<V>, pivotTable: seq<Key>) : (s : Option<seq<Bucket>>)
-  requires Pivots.WFPivots(pivotTable)
-  requires forall i | 0 <= i < |a| :: ValidVal(a[i])
-  requires forall i | 0 <= i < |a| :: ValInGrammar(a[i], BucketGrammar())
-  requires |a| <= |pivotTable| + 1
-  ensures s.Some? ==> |s.value| == |a|
-  ensures s.Some? ==> forall i | 0 <= i < |s.value| :: WFBucketAt(s.value[i], pivotTable, i)
-  {
-    if |a| == 0 then
-      Some([])
-    else (
-      match valToBuckets(DropLast(a), pivotTable) {
-        case None => None
-        case Some(pref) => (
-          match valToBucket(Last(a), pivotTable, |pref|) {
-            case Some(bucket) => Some(pref + [KVList.I(bucket)])
-            case None => None
-          }
-        )
-      }
-    )
-  }
-
-  function {:fuel ValInGrammar,2} valToNode(v: V) : (s : Option<Node>)
-  requires ValidVal(v)
-  requires ValInGrammar(v, PivotNodeGrammar())
-  // Pivots.NumBuckets(node.pivotTable) == |node.buckets|
-  ensures s.Some? ==> SM.WFNode(s.value)
-  ensures s.Some? ==> BT.WFNode(SM.INode(s.value))
-  {
-    assert ValidVal(v.t[0]);
-    assert ValidVal(v.t[1]);
-    assert ValidVal(v.t[2]);
-    var pivots_len := |v.t[0].baa| as uint64;
-    var children_len := |v.t[1].ua| as uint64;
-    var buckets_len := |v.t[2].a| as uint64;
-
-    if (
-       && pivots_len <= MaxNumChildrenUint64() - 1
-       && (children_len == 0 || children_len == pivots_len + 1)
-       && buckets_len == pivots_len + 1
-    ) then (
-      assert ValidVal(v.t[0]);
-      match valToPivots(v.t[0]) {
-        case None => None
-        case Some(pivots) => (
-          match valToChildren(v.t[1]) {
-            case None => None
-            case Some(children) => (
-              assert ValidVal(v.t[2]);
-              match valToBuckets(v.t[2].a, pivots) {
-                case None => None
-                case Some(buckets) => (
-                  if WeightBucketList(buckets) <= MaxTotalBucketWeight() then (
-                    var node := SM.Node(
-                      pivots,
-                      if |children| == 0 then None else Some(children),
-                      buckets);
-                    Some(node)
-                  ) else (
-                    None
-                  )
-                )
-              }
-            )
-          }
-        )
-      }
-    ) else (
-      None
-    )
-  }
-
-  function valToSector(v: V) : (s : Option<Sector>)
-  requires ValidVal(v)
-  requires ValInGrammar(v, SectorGrammar())
-  {
-    if v.c == 0 then (
-      match IndirectionTableModel.valToIndirectionTable(v.val) {
-        case Some(s) => Some(SM.SectorIndirectionTable(s))
-        case None => None
-      }
-    ) else (
-      match valToNode(v.val) {
-        case Some(s) => Some(SM.SectorBlock(s))
-        case None => None
-      }
-    )
-  }
-
   /////// Some lemmas that are useful in Impl
 
   lemma WeightBucketLteSize(v: V, pivotTable: seq<Key>, i: int, kvl: KVList.Kvl)
-  requires valToBucket.requires(v, pivotTable, i)
-  requires valToBucket(v, pivotTable, i) == Some(kvl)
+  requires Marshalling.valToBucket.requires(v, pivotTable, i)
+  requires Marshalling.valToBucket(v, pivotTable, i) == Some(kvl)
   ensures WeightBucket(KVList.I(kvl)) <= SizeOfV(v)
   {
     KVList.kvlWeightEq(kvl);
@@ -329,8 +76,8 @@ module ImplMarshallingModel {
 
   lemma WeightBucketListLteSize(v: V, pivotTable: seq<Key>, buckets: seq<Bucket>)
   requires v.VArray?
-  requires valToBuckets.requires(v.a, pivotTable)
-  requires valToBuckets(v.a, pivotTable) == Some(buckets)
+  requires Marshalling.valToBuckets.requires(v.a, pivotTable)
+  requires Marshalling.valToBuckets(v.a, pivotTable) == Some(buckets)
   ensures WeightBucketList(buckets) <= SizeOfV(v)
 
   decreases |v.a|
@@ -341,8 +88,8 @@ module ImplMarshallingModel {
       WeightBucketListLteSize(VArray(DropLast(v.a)), pivotTable, DropLast(buckets));
       lemma_SeqSum_prefix(DropLast(v.a), Last(v.a));
 
-      var pref := valToBuckets(DropLast(v.a), pivotTable).value;
-      var kvl := valToBucket(Last(v.a), pivotTable, |pref|).value;
+      var pref := Marshalling.valToBuckets(DropLast(v.a), pivotTable).value;
+      var kvl := Marshalling.valToBucket(Last(v.a), pivotTable, |pref|).value;
       WeightBucketLteSize(Last(v.a), pivotTable, |pref|, kvl);
 
       assert DropLast(v.a) + [Last(v.a)] == v.a;
@@ -408,7 +155,40 @@ module ImplMarshallingModel {
     VUint64(lba)
   }
 
+  function {:fuel ValInGrammar,2} valToNode(v: V) : (s : Option<Node>)
+  requires ValidVal(v)
+  requires ValInGrammar(v, Marshalling.PivotNodeGrammar())
+  ensures s.Some? ==> SM.WFNode(s.value)
+  ensures s.Some? ==> BT.WFNode(SM.INode(s.value))
+  {
+    // TODO(travis): is there any reason to SM.Node be a different
+    // type than BC.G.Node?
+    var node := Marshalling.valToNode(v);
+    if node.Some? then (
+      Some(SM.Node(node.value.pivotTable, node.value.children, node.value.buckets))
+    ) else (
+      None
+    )
+  }
+
   /////// Marshalling and de-marshalling
+
+  function valToSector(v: V) : (s : Option<Sector>)
+  requires ValidVal(v)
+  requires ValInGrammar(v, Marshalling.SectorGrammar())
+  {
+    if v.c == 0 then (
+      match IndirectionTableModel.valToIndirectionTable(v.val) {
+        case Some(s) => Some(SM.SectorIndirectionTable(s))
+        case None => None
+      }
+    ) else (
+      match valToNode(v.val) {
+        case Some(s) => Some(SM.SectorBlock(s))
+        case None => None
+      }
+    )
+  }
 
   function {:opaque} parseSector(data: seq<byte>) : (s : Option<Sector>)
   ensures s.Some? ==> SM.WFSector(s.value)
@@ -416,7 +196,7 @@ module ImplMarshallingModel {
       IndirectionTableModel.TrackingGarbage(s.value.indirectionTable)
   {
     if |data| < 0x1_0000_0000_0000_0000 then (
-      match parse_Val(data, SectorGrammar()).0 {
+      match parse_Val(data, Marshalling.SectorGrammar()).0 {
         case Some(v) => valToSector(v)
         case None => None
       }
@@ -437,4 +217,5 @@ module ImplMarshallingModel {
     else
       None
   }
+
 }
